notation ok for the while

reinvent/grp01.v
@@ -14,39 +14,42 @@ Structure Setoid : Type := {
 #[global]
 Existing Instance setoid_prf.
 
-Notation "[ 'setoid' 'by' P 'on' A ]" := (@Build_Setoid A P _).
-Notation "[ 'setoid' 'by' P ]" := [setoid by P on _].
-Notation "(== 'in' A )" := (setoid_equal A).
+Notation "'std' 'by' P 'on' A " := (@Build_Setoid A P _)
+  (at level 100, P at next level, no associativity) : setoid_scope.
+Notation "'std' 'by' P" := (std by P on _)
+  (at level 100, no associativity) : setoid_scope.
+Notation "( == 'in' A )" := (setoid_equal A)
+  (at level 0, format "( == 'in' A )").
 Notation "x == y 'in' A" := (setoid_equal A x y)
   (at level 70, y at next level, no associativity).
 Notation "(==)" := (== in _).
-Notation "x == y" := (x == y in _) (at level 70, no associativity).
+Notation "x == y" := (x == y in _)
+  (at level 70, no associativity) : setoid_scope.
 Notation typeof := setoid_carrier.
 
-Program Definition eq_setoid (X:Type) := [setoid by @eq X].
+Program Definition eqSetoid (X:Type) := std by @eq X.
 
-Program Definition function (X Y:Type) : Setoid :=
-  [setoid by `(forall x, f x = g x) on X -> Y].
+Program Definition functionSetoid (X Y:Type) : Setoid :=
+  std by `(forall x, f x = g x) on (X -> Y).
 Next Obligation. split; intros x; congruence. Defined.
-Canonical Structure function.
+Canonical Structure functionSetoid.
 
-Program Definition prop_setoid := [setoid by iff].
-Canonical Structure prop_setoid.
+Program Definition PropSetoid := std by iff.
+Canonical Structure PropSetoid.
 
 Inductive empty : Type := .
-Program Definition empty_setoid :=
-  [setoid by fun e e' => match e, e' with end on empty].
+Program Definition emptySetoid :=
+  std by fun e e' => match e, e' with end on empty.
 Next Obligation. split; intros x; case x. Qed.
 
-Program Definition unit_setoid :=
-  [setoid by fun _ _ => True on unit].
+Program Definition unitSetoid := std by fun _ _ => True on unit.
 Next Obligation. split; intros H; tauto. Qed.
 
-Definition prod_eq {A B:Setoid} (a b: A * B) :=
+Definition DirectProduct_eq {A B:Setoid} (a b: A * B) :=
    fst a == fst b /\ snd a == snd b.
 
-Program Definition dprod_setoid (A B:Setoid) :=
-  [setoid by prod_eq on A * B].
+Program Definition DirectProductSetoid (A B:Setoid) :=
+  std by DirectProduct_eq on A * B.
 Next Obligation.
   split.
   - intros a. now split.
@@ -54,8 +57,9 @@ Next Obligation.
   - intros a b c [H1 H2] [H3 H4]. split;
     now (rewrite H1, H3 || rewrite H2, H4).
 Defined.
-Canonical Structure dprod_setoid.
-Notation "[ 'dprodstd' A \* B ]" := (dprod_setoid A B) : setoid_scope.
+Canonical Structure DirectProductSetoid.
+Notation "[( A , B )]" := (DirectProductSetoid A B)
+  : setoid_scope.
 
 
 Class IsSubsetoid (X:Setoid) (conf: typeof X -> Prop) := {
@@ -70,39 +74,44 @@ Structure Subsetoid (X:Setoid) : Type := {
 #[global]
 Existing Instance sub_prf.
 
-Notation "[ 'substd' 'by' C 'on' A ]" := (@Build_Subsetoid A C _).
-Notation "[ 'substd' 'by' C ]" := [substd by C on _].
-Notation "[ 'substd' 'of' x 'in' A | P ]" := [substd by (fun x => P) on A].
-Notation "[ 'substd' 'of' x | P ]" := [substd of x in _ | P].
+Notation "'sstd' 'by' C 'on' A" := (@Build_Subsetoid A C _)
+  (at level 100, C at next level, no associativity) : setoid_scope.
+Notation "'sstd' 'by' C" := (sstd by C on _)
+  (at level 100, no associativity) : setoid_scope.
+Notation "[  x 'in' A | P  ]" := (sstd by (fun x => P) on A)
+  : setoid_scope.
+Notation "[  x | P  ]" := [x in _ | P]
+  : setoid_scope.
 
-Program Coercion subsetoid_to_setoid `(B: Subsetoid A) :=
-  [setoid by (== in A) on {x|B x}].
+Program Coercion Subsetoid_toSetoid `(B: Subsetoid A) :=
+  std by (== in A) on { x | B x }.
 Next Obligation.
   split.
   - now intros x.
   - intros x y Heq. now symmetry.
   - intros x y z Heq1 Heq2. now rewrite Heq1.
 Defined.
-Notation "[| B |]" := (subsetoid_to_setoid B) : setoid_scope.
-Notation "[| 'substd' 'by' C 'on' A |]" := [|[substd by C on A]|].
-Notation "[| 'substd' 'by' C |]" := [|[substd by C]|].
-Notation "[| 'substd' 'of' x 'in' A | P |]" := [|[substd by (fun x => P) on A]|].
-Notation "[| 'substd' 'of' x | P |]" := [|[substd of x | P]|].
+Notation "[|  B  |]" := (@Subsetoid_toSetoid _ B) : setoid_scope.
 
-Program Definition self_substd (A:Setoid) := [substd of x | True].
+
+Program Definition selfSubsetoid (A:Setoid) := [ _ | True ].
 Next Obligation. split. now intros x y Heq. Defined.
-Notation "[{ A }]" := (self_substd A) : setoid_scope.
+Notation "[{  A  }]" := (@selfSubsetoid A) : setoid_scope.
 
-Program Definition empty_subsetoid (A:Setoid) := [substd of x | False].
+Program Definition emptySubsetoid {A:Setoid} := [ _ | False ].
 Next Obligation. split. now intros x y Heq. Defined.
+Notation "[{ } 'in' A  ]" := (@emptySubsetoid A) : setoid_scope.
+Notation "[{ }]" := [{} in _] : setoid_scope.
 
-Program Definition solo_substd {A:Setoid} (a:A) 
-  := [substd of x | x == a].
+Program Definition unitSubsetoid {A:Setoid} (a:A) 
+  := [ x | x == a ].
 Next Obligation.
   split. intros x y Heq. split; intros Heq1; now rewrite <-Heq1.
 Defined.
-Notation "[$ a 'in' A ]" := (@solo_substd A a).
-Notation "[$ a ]" := [$a in _].
+Notation "[  $ a 'in' A  ]" := (@unitSubsetoid A a)
+  : setoid_scope.
+Notation "[  $ a  ]" := [ $ a in _]
+  : setoid_scope.
 
 
 Class Included {X} (A B: Subsetoid X) := {
@@ -110,13 +119,13 @@ Class Included {X} (A B: Subsetoid X) := {
 }.
 Notation "A '<=' B" := (@Included _ A B) : setoid_scope.
 
-Lemma included_transitive {X} : Transitive (@Included X).
+Lemma included_trans {X} : Transitive (@Included X).
 Proof. split. intros a xa. apply H0, H, xa. Qed.
 #[global]
-Existing Instance included_transitive.
+Existing Instance included_trans.
 
-Program Definition Subsetoid_setoid (X:Setoid) :=
-  [setoid by fun A B => A <= B /\ B <= A on Subsetoid X].
+Program Definition SubsetoidSetoid (X:Setoid) :=
+  std by fun A B => A <= B /\ B <= A on Subsetoid X.
 Next Obligation.
   split.
   - intros A. split; split; intros x Ax; apply Ax.
@@ -125,7 +134,7 @@ Next Obligation.
     + intros Ax. apply BC. now apply AB.
     + intros Cx. apply BA. now apply CB.
 Defined.
-Canonical Structure Subsetoid_setoid.
+Canonical Structure SubsetoidSetoid.
 
 Class IsMap {X Y:Setoid} (f: X -> Y) := {
   map_proper:> Proper ((==) ==> (==)) f
@@ -139,17 +148,19 @@ Structure Map (X Y:Setoid) : Type := {
 #[global]
 Existing Instance map_prf.
 
-Notation "[ 'map' 'by' f ]" := (@Build_Map _ _ f _) : setoid_scope.
-Notation " 'map' x 'in' X => m " := [map by fun (x:X) => m]
-  (at level 70, right associativity) : setoid_scope.
+Notation "'map' 'by' f" := (@Build_Map _ _ f _)
+  (at level 100, no associativity) : setoid_scope.
+Notation " 'map' x 'in' X => m " := (map by fun (x:X) => m)
+  (at level 100, x, X at next level, no associativity)
+   : setoid_scope.
 Notation " 'map' x => m " := (map x in _ => m)
-  (at level 70, right associativity) : setoid_scope.
+  (at level 100, x at next level, no associativity) : setoid_scope.
 
 Program Definition Map_id {X:Setoid} : Map X X := map x => x.
 Next Obligation. split. intros x y Heq. apply Heq. Defined.
 
-Program Definition Map_setoid (X Y: Setoid) : Setoid :=
-  [setoid by ((==) ==> (==))%signature on Map X Y].
+Program Definition MapSetoid (X Y: Setoid) : Setoid :=
+  std by ((==) ==> (==))%signature on Map X Y.
 Next Obligation.
   split.
   - intros f x y Heq. now rewrite Heq. 
@@ -157,7 +168,7 @@ Next Obligation.
   - intros f g h Heq1 Heq2 x y Heq3. 
     now rewrite (Heq1 x y Heq3), <-(Heq2 x y Heq3), Heq3.
 Defined.
-Canonical Structure Map_setoid.
+Canonical Structure MapSetoid.
 
 Program Definition Map_compose {X Y Z} (f: Map X Y) (g: Map Y Z)
   : Map X Z := map x => g (f x).
@@ -179,7 +190,7 @@ Class Bijective `(f: Map X Y) : Prop := {
   bij_surjective:> Surjective f
 }.
 
-Lemma mapcomp_reduc : forall {X Y Z} {f g: Map Y Z} {h: Map X Y},
+Lemma Map_reduc : forall {X Y Z} {f g: Map Y Z} {h: Map X Y},
   Surjective h -> f \o h == g \o h -> f == g.
 Proof.
   intros X Y Z f g h [Sh] Heq. simpl. intros x y Heq1.
@@ -187,14 +198,14 @@ Proof.
   rewrite Heq2. now apply Heq.
 Qed.
 
-Lemma mapcomp_assoc {X Y Z W} {f: Map Z W} {g: Map Y Z} {h: Map X Y} :
+Lemma Map_assoc {X Y Z W} {f: Map Z W} {g: Map Y Z} {h: Map X Y} :
   (f \o g) \o h == f \o g \o h.
 Proof. intros. simpl. intros x y Heq. now rewrite Heq. Qed.
 
 
 Program Definition Image `(f: Map X Y)
-  : Map (Subsetoid_setoid X) (Subsetoid_setoid Y)
-  := map A => [substd of y | exists x, A x /\ y == f x].
+  : Map (Subsetoid X) (Subsetoid Y)
+  := map A => [ y | exists x, A x /\ y == f x ].
 Next Obligation.
   split. intros a b Heq. split; intros [x [Ax Heq1]]; exists x;
   split; try apply Ax; (now rewrite <-Heq || now rewrite Heq).
@@ -207,8 +218,8 @@ Next Obligation.
 Defined.
 
 Program Definition Preimage `(f: Map X Y)
-  : Map (Subsetoid_setoid Y) (Subsetoid_setoid X)
-  := map B => [substd of x | B (f x)].
+  : Map (Subsetoid Y) (Subsetoid X)
+  := map B => [ x | B (f x) ].
 Next Obligation. split. intros a b Heq. now rewrite Heq. Defined.
 Next Obligation.
   split. intros A B [AB BA]. split; split; simpl;
@@ -216,11 +227,11 @@ Next Obligation.
 Defined.
 
 
-Program Definition inclusion `{B: Subsetoid A} : Map [|B|] A
+Program Definition inclusion `{B: Subsetoid A} : Map B A
   := map h => h.
 Next Obligation. split. intros x y. now simpl. Defined.
 
-Lemma inc_inj `{B: Subsetoid A} : Injective (@inclusion A B).
+Lemma inclusion_inj `{B: Subsetoid A} : Injective (@inclusion A B).
 Proof. split. intros x y. now simpl. Qed.
 
 
@@ -239,11 +250,12 @@ Structure Binop (X:Setoid) := {
 #[global]
 Existing Instance binop_prf.
 
-Notation "[ 'binop' 'by' f ]" := (@Build_Binop _ f _) : alg_scope.
-Notation " 'binop' x , y 'in' A => m " := [binop by fun (x y:A) => m]
-  (at level 70, right associativity) : alg_scope.
-Notation " 'binop' x , y => m " := [binop by fun (x y:_) => m]
-  (at level 70, right associativity) : alg_scope.
+Notation "'binop' 'by' f" := (@Build_Binop _ f _)
+  (at level 100, no associativity) : alg_scope.
+Notation " 'binop' x , y 'in' A => m " := (binop by fun (x y:A) => m)
+  (at level 100, x, y, A at next level, no associativity) : alg_scope.
+Notation " 'binop' x , y => m " := (binop by fun (x y:_) => m)
+  (at level 100, x, y at next level, no associativity) : alg_scope.
 
 
 Class Associative `(op: Binop X) := {
@@ -282,18 +294,20 @@ Structure Monoid := {
 #[global]
 Existing Instance monoid_prf.
 
-Notation "[ 'monoid' 'by' op , id 'on' A ]" :=
-  (@Build_Monoid A op id _) : alg_scope.
-Notation "[ 'monoid 'by' op , id ]" :=
-  [monoid by op, id on _] : alg_scope.
+Notation "'mnd' 'by' op , id 'on' A" := (@Build_Monoid A op id _)
+  (at level 100, op, id at next level, no associativity) : alg_scope.
+Notation "'mnd' 'by' op , id" := (mnd by op, id on _)
+  (at level 100, op, id at next level, no associativity) : alg_scope.
 
 
 Class LInvertible `(op: Binop X) (e:X) (inv: Map X X) := {
   linvertible: forall x, op (inv x) x == e
 }.
+
 Class RInvertible `(op: Binop X) (e:X) (inv: Map X X) := {
   rinvertible: forall x, op x (inv x) == e
 }.
+
 Class Invertible `(op: Binop X) (e:X) (inv: Map X X) := {
   invertible_l:> LInvertible op e inv;
   invertible_r:> RInvertible op e inv
@@ -321,30 +335,32 @@ Structure Group := {
 #[global]
 Existing Instance grp_prf.
 
-Notation "[ 'group' 'by' op , inv , id 'on' A ]" :=
-  (@Build_Group A op inv id _).
-Notation "[ 'group' 'by' op , inv , id ]" := [group by op, inv, id on _].
-Notation "( * 'in' G )" := (@grp_op G) : alg_scope.
-Notation "( * )" := ( * in _) : alg_scope.
+Notation "'grp' 'by' op , inv , id 'on' A" :=
+  (@Build_Group A op inv id _)
+  (at level 100, op, inv, id at next level, no associativity) : alg_scope.
+Notation "'grp' 'by' op , inv , id" := (grp by op, inv, id on _)
+  (at level 100, op, inv, id at next level, no associativity) : alg_scope.
+Notation "( * 'in' G  )" := (@grp_op G) : alg_scope.
+Notation "( * )" := ( * in _ ) : alg_scope.
 Notation "g *_{ G } h" := (@grp_op G g h)
-  (at level 60, right associativity) : alg_scope.
+  (at level 40, left associativity) : alg_scope.
 Notation "g * h" := (g *_{_} h) : alg_scope.
 Notation "1_{ G }" := (@grp_id G) : alg_scope.
 Notation "'1'" := 1_{_} : alg_scope.
-Notation "(\! 'in' G ) " := (@grp_inv G) : alg_scope.
-Notation "(\!)" := (\! in _) : alg_scope.
+Notation "( ! 'in' G  ) " := (@grp_inv G) : alg_scope.
+Notation "( ! )" := ( ! in _) : alg_scope.
 Notation "!_{ G } g " := (@grp_inv G g)
-  (at level 30, right associativity) : alg_scope.
+  (at level 35, right associativity) : alg_scope.
 Notation "! g" := ( !_{_} g)
-  (at level 8, right associativity) : alg_scope.
+  (at level 35, right associativity) : alg_scope.
 
-Lemma grp_id_ident_l : forall {G:Group}, LIdentical ( * in G) 1.
+Lemma grp_id_ident_l : forall {G:Group}, LIdentical ( * in G ) 1.
 Proof.
   split. intros x.
   assert (1 * x == 1 * (x * 1)) as Heq0.
   { now rewrite ridentical. }
   assert (x * 1 == x * !x * !!x) as Heq1.
-  { now rewrite <-(rinvertible !x), associative. }
+  { now rewrite <-(rinvertible (!x)), associative. }
   rewrite Heq0, Heq1, rinvertible, associative, ridentical.
   assert (1 == x * !x) as Heq2. { now rewrite rinvertible. }
   now rewrite Heq2, <-associative, rinvertible, ridentical.
@@ -352,7 +368,7 @@ Qed.
 #[global]
 Existing Instance grp_id_ident_l.
 
-Lemma grp_inv_invert_l {G} : LInvertible ( * in G) 1 (\!).
+Lemma grp_inv_invert_l {G} : LInvertible ( * in G) 1 ( ! ).
 Proof.
   split. intros x.
   assert (!x * x == !x * (x * !x) * !!x) as Heq0.
@@ -364,7 +380,7 @@ Existing Instance grp_inv_invert_l.
 
 Section GroupTheory.
   Context {G:Group}.
-  Lemma grp_op_inj_r : forall {g x y:G},
+  Lemma opinj_r : forall {g x y:G},
     x * g == y * g -> x == y.
   Proof.
     intros g x y Heq.
@@ -373,7 +389,7 @@ Section GroupTheory.
     now rewrite rinvertible, 2!ridentical in H.
   Qed.
 
-  Lemma grp_op_inj_l : forall {g x y:G},
+  Lemma opinj_l : forall {g x y:G},
     g * x == g * y -> x == y.
   Proof.
     intros g x y Heq. 
@@ -382,55 +398,43 @@ Section GroupTheory.
     now rewrite linvertible, 2!lidentical in H.
   Qed.
 
-  Lemma grp_op_feq_l : forall {g x y:G},
-    x == y -> g * x == g * y.
-  Proof.
-    intros g x y Heq. now rewrite Heq.
-  Qed.
-
-  Lemma grp_op_feq_r : forall {g x y:G},
-    x == y -> x * g == y * g.
-  Proof.
-    intros g x y Heq. now rewrite Heq.
-  Qed.
-
-  Lemma grp_send_l : forall {g x y:G},
+  Lemma send_l : forall {g x y:G},
     g * x == y -> x == !g * y.
   Proof.
     intros g x y Heq.
-    apply (grp_op_inj_l(g:=g)).
+    apply (opinj_l(g:=g)).
     now rewrite associative, rinvertible, lidentical.
   Qed.
 
-  Lemma grp_send_r : forall {g x y:G},
+  Lemma send_r : forall {g x y:G},
     x * g == y -> x == y * !g.
   Proof.
     intros g x y Heq.
-    apply (grp_op_inj_r(g:=g)).
+    apply (opinj_r(g:=g)).
     now rewrite <-associative, linvertible, ridentical.
   Qed.
 
-  Lemma grp_invinv : forall {x:G}, !!x == x.
+  Lemma invinv : forall {x:G}, !!x == x.
   Proof.
     intros x.
     assert (!!x * !x == x * !x) as H.
     { now rewrite linvertible, rinvertible. }
-    now apply grp_op_inj_r in H.
+    now apply opinj_r in H.
   Qed.
 
-  Lemma grp_opinv : forall {x y:G},
+  Lemma opinv : forall {x y:G},
     !(x * y) == !y * !x.
   Proof.
     intros x y. 
     rewrite <-(ridentical (!y * !x)), <-associative.
-    apply grp_send_l, grp_send_l.
+    apply send_l, send_l.
     now rewrite associative, rinvertible.
   Qed.
 
-  Lemma grp_invid_id : !1_{G} == 1.
+  Lemma invid : !1_{G} == 1.
   Proof.
-    rewrite <-(ridentical !1).
-    symmetry; apply grp_send_l, lidentical.
+    rewrite <-(ridentical (!1)).
+    symmetry; apply send_l, lidentical.
   Qed.
 End GroupTheory.
 
@@ -448,12 +452,14 @@ Structure Homomorph (G H:Group) := {
 #[global]
 Existing Instance hom_prf.
 
-Notation "[ 'hom' 'by' f ]" :=
-  (@Build_Homomorph _ _ [map by f] _) : alg_scope.
-Notation " 'hom' x 'in' G => m " := [hom by fun (x:G) => m]
-  (at level 70, right associativity) : alg_scope.
+Notation "'hom' 'besides' 'map' f" := (@Build_Homomorph _ _ f _)
+  (at level 100, no associativity) : alg_scope.
+Notation "'hom' 'by' f " := (hom besides map (map by f))
+  (at level 100, no associativity) : alg_scope.
+Notation " 'hom' x 'in' G => m " := (hom by fun (x:G) => m)
+  (at level 100, x, G at next level, no associativity) : alg_scope.
 Notation " 'hom' x => m " := (hom x in _ => m)
-  (at level 70, right associativity) : alg_scope.
+  (at level 100, x at next level, no associativity) : alg_scope.
 
 Class IsIsomorph `(f: Homomorph G H) := {
   isomorph:> Bijective f
@@ -467,34 +473,38 @@ Structure Isomorph (G H:Group):= {
 #[global]
 Existing Instance iso_prf.
 
-Notation "[ 'iso' 'by' f ]" :=
-  (@Build_Isomorph _ _ [hom by f] _) : alg_scope.
-Notation "'iso' x 'in' G => m " := [iso by fun (x:G) => m]
-  (at level 70, right associativity) : alg_scope.
+Notation "'iso' 'besides' 'hom' f" := (@Build_Isomorph _ _ f _)
+  (at level 100, no associativity) : alg_scope.
+Notation "'iso' 'besides' 'map' f" := (iso besides hom (hom besides map f))
+  (at level 100, no associativity) : alg_scope.
+Notation "'iso' 'by' f" := (iso besides hom (hom by f))
+  (at level 100, no associativity) : alg_scope.
+Notation "'iso' x 'in' G => m " := (iso by fun (x:G) => m)
+  (at level 100, x, G at next level, no associativity) : alg_scope.
 Notation "'iso' x => m " := (iso x in _ => m)
-  (at level 70, right associativity) : alg_scope.
+  (at level 100, x at next level, no associativity) : alg_scope.
 Notation "G ~= H" := (Isomorph G H)
-  (at level 60, right associativity) : alg_scope.
+  (at level 95, right associativity) : alg_scope.
 
 Program Definition Hom_compose {X Y Z:Group}
   (f: Homomorph X Y) (g: Homomorph Y Z)
-  : Homomorph X Z := Build_Homomorph _ _ (g \o f) _.
+  : Homomorph X Z := hom besides map (g \o f).
 Next Obligation.
   split. intros x y. simpl. now rewrite 2!homomorph.
 Defined.
-Notation "g \o_h f" := (Hom_compose f g)
+Notation "g 'hom\o' f" := (Hom_compose f g)
   (at level 60, right associativity) : alg_scope.
 
 Program Definition Iso_compose {X Y Z:Group}
   (f: Isomorph X Y) (g: Isomorph Y Z)
-  : Isomorph X Z := Build_Isomorph _ _ (g \o_h f) _.
+  : Isomorph X Z := iso besides hom (g hom\o f).
 Next Obligation.
   split; split; split; simpl.
   - intros x y Heq. now apply injective, injective in Heq.
   - intros y. destruct (surjective y). destruct (surjective x).
     exists x0. now rewrite <-H0, <-H.
 Defined.
-Notation "g \o_i f" := (Iso_compose f g)
+Notation "g 'iso\o' f" := (Iso_compose f g)
   (at level 60, right associativity) : alg_scope.
 
 
@@ -503,25 +513,25 @@ Section HomTheory.
   Lemma hom_id : f 1 == 1.
   Proof.
     rewrite <-(rinvertible (f 1)).
-    apply grp_send_r. now rewrite <-homomorph, ridentical.
+    apply send_r. now rewrite <-homomorph, ridentical.
   Qed.
 
-  Lemma hom_inv : forall x, f !x == !(f x).
+  Lemma hom_inv : forall x, f (!x) == !(f x).
   Proof.
     intros x.
-    rewrite <-(ridentical !(f x)).
-    apply grp_send_l.
+    rewrite <-(ridentical (!(f x))).
+    apply send_l.
     now rewrite <-homomorph, rinvertible, hom_id.
   Qed.
 End HomTheory.
 
 
 Class IsSubgroup (G:Group) (H: Subsetoid G) := {
-  sg_ferm_op:
+  ferm_op:
     forall {x y}, H x -> H y -> H (x * y);  
-  sg_ferm_inv:
-    forall {x}, H x -> H !x;
-  sg_ferm_id: H 1
+  ferm_inv:
+    forall {x}, H x -> H (!x);
+  ferm_id: H 1
 }.
 
 Structure Subgroup (G:Group) := {
@@ -535,29 +545,29 @@ Existing Instance sg_prf.
 Arguments sg_supp {_} _.
 
 Notation "H '<-' G" := (IsSubgroup G H)
-  (at level 60, right associativity) : alg_scope.
+  (at level 70, no associativity) : alg_scope.
 Notation "H <<- G" := (@Build_Subgroup G H _)
-  (at level 60, right associativity) : alg_scope.
+  (at level 70, no associativity) : alg_scope.
 
-Program Coercion sg_as_group `(H:Subgroup G) :=
-  [group by (binop x, y => x * y), (map x => !x), 1 on [|H|]].
-Next Obligation. apply sg_ferm_op; (apply H1 || apply H0). Defined.
+Program Coercion Subgroup_toGroup `(H:Subgroup G) :=
+  grp by (binop x, y => x * y), (map x => !x), 1 on H.
+Next Obligation. apply ferm_op; (apply H1 || apply H0). Defined.
 Next Obligation.
   split. intros x1 y1 Heq x0 y0 Heq1. simpl.
   simpl in Heq. simpl in Heq1. now rewrite Heq, Heq1.
 Defined.
-Next Obligation. apply sg_ferm_inv, H0. Defined.
+Next Obligation. apply ferm_inv, H0. Defined.
 Next Obligation.
   split. intros x y. simpl. intros Heq. now rewrite Heq.
 Defined.
-Next Obligation. apply sg_ferm_id. Defined.
+Next Obligation. apply ferm_id. Defined.
 Next Obligation.
   split.
   - split. intros x y z. simpl. apply associative.
   - split. intros x. simpl. apply ridentical.
   - split. intros x. simpl. apply rinvertible.
 Defined.
-Notation "[ 'grp' | H |]" := (@sg_as_group _ H).
+Notation "<|  H  |>" := (@Subgroup_toGroup _ H).
 
 Class IsNormalSubgroup `(H: Subgroup G) := {
   normal:
@@ -573,17 +583,17 @@ Structure NormalSubgroup (G:Group):= {
 Existing Instance nsg_prf.
 
 Notation "H <| G" := (@IsNormalSubgroup G H)
-  (at level 60, right associativity) : alg_scope.
+  (at level 70, no associativity) : alg_scope.
 Notation "H <<| G" :=
   (@Build_NormalSubgroup G H _)
-  (at level 60, right associativity) : alg_scope.
+  (at level 70, no associativity) : alg_scope.
 Notation "H <<-| G" :=
   (@Build_NormalSubgroup G (H <<- G) _)
-  (at level 60, right associativity) : alg_scope.
+  (at level 70, no associativity) : alg_scope.
 
 
-Program Definition Subgroupable_subsetoid (G:Group) :=
-  [substd of H in Subsetoid_setoid G | H <- G].
+Program Definition GroupableSubsetoid (G:Group) :=
+  [ H in Subsetoid G | H <- G].
 Next Obligation.
   split. intros H1 H2. simpl. intros [H1H2 H2H1]. split;
   intros [Hfop Hfinv Hfid]; split; try intros x y Hx Hy;
@@ -593,81 +603,93 @@ Next Obligation.
   try apply Hfid; try apply Hfop; try apply Hfinv;
   try apply H1H2; try apply Hx; try apply Hy.
 Defined.
-Notation "[ 'grpables' 'of' G ]" := [|Subgroupable_subsetoid G|].
+Notation "[ | <- G  ]" := (@GroupableSubsetoid G).
 
-Program Definition _sgstd_as_sg `(H: [grpables of G])
-  : Subgroup G :=  H <<- G.
-
-
-Program Definition Subgroup_setoid (G:Group) :=
-  [setoid by (== in Subsetoid G) on Subgroup G].
+Program Definition SubgroupSetoid (G:Group) :=
+  std by (== in Subsetoid G) on Subgroup G.
 Next Obligation.
   split; try now intros x.
   intros x y z [Hxy Hyx] [Hyz Hzy]. split.
   - apply (transitivity Hxy Hyz).
   - apply (transitivity Hzy Hyx).
 Defined.
-Canonical Structure Subgroup_setoid.
+Canonical Structure SubgroupSetoid.
+Notation "[ <> | <- G  ]" := (SubgroupSetoid G). 
 
-Program Definition grpable_as_sg {G:Group}
-  : Map [grpables of G] (Subgroup G)
+Program Definition GroupableSubsetoid_toSubgroup {G:Group}
+  : Map [ | <- G ] [ <> | <- G ]
   := map H => H <<- G.
 Next Obligation. split. intros A B. simpl. intuition. Defined.
+Notation "H <<[]- G" :=
+  (@GroupableSubsetoid_toSubgroup G H)
+  (at level 70, no associativity) : alg_scope.
 
-Program Definition sg_as_grpable {G:Group}
-  : Map (Subgroup G) [grpables of G]
+Program Definition Subgroup_toGroupableSetoid {G:Group}
+  : Map [ <> | <- G ] [ | <- G ]
   := map H => sg_supp H.
 Next Obligation. intuition. Defined.
 Next Obligation. split. intros A B. simpl. intuition. Defined.
+Notation "H [<-] G" :=
+  (@Subgroup_toGroupableSetoid G H)
+  (at level 70, no associativity) : alg_scope.
 
 
-Program Definition sg_self (G:Group) : Subgroup G := [{G}] <<- G.
+Program Definition selfSubgroup (G:Group) : Subgroup G
+  := [{ G }] <<- G.
 Next Obligation. split; simpl; intros; trivial. Defined.
-Notation "[ 'subgrp' { G }]" := (sg_self G).
+Notation "<{ G }>" := (selfSubgroup G).
 
-Program Definition sg_id {G:Group}
+Program Definition idNormalSubgroup {G:Group}
   : NormalSubgroup G := [$1] <<-| G.
 Next Obligation. 
   split; simpl; intuition.
   - rewrite H, H0. apply lidentical.
-  - rewrite H. apply grp_invid_id.
+  - rewrite H. apply invid.
 Defined.
 Next Obligation.
   split. intros g h. simpl. intros Heq.
   now rewrite Heq, ridentical, rinvertible.
 Defined.
+Notation "< 1 'in' G  >" := (@idNormalSubgroup G)
+  (at level 0, G at next level)
+  : alg_scope.
+Notation "<1>" := < 1 in _ >
+  : alg_scope.
 
-Program Definition sg_in_sg {G:Group} (N H: Subgroup G)
-  : Subgroup H := [substd of n | N n] <<- H.
+Program Definition Subgroup_inSubgroup {G:Group} (N H: Subgroup G)
+  : Subgroup H := [ n | N n ] <<- H.
 Next Obligation. split. intros g h. simpl. intros Heq. now rewrite Heq. Defined.
 Next Obligation.
   split; simpl.
-  - intros x y Nx Ny. apply (sg_ferm_op Nx Ny).
-  - intros x Nx. apply (sg_ferm_inv Nx).
-  - apply sg_ferm_id. 
+  - intros x y Nx Ny. apply (ferm_op Nx Ny).
+  - intros x Nx. apply (ferm_inv Nx).
+  - apply ferm_id. 
 Defined.
-Notation "[ 'subgrp' N 'in' H ]" := (@sg_in_sg _ N H).
+Notation "<  N 'inside' H   >" := (@Subgroup_inSubgroup _ N H)
+  (at level 0, N, H at next level)
+  : alg_scope.
 
-Program Definition nsg_in_sg {G:Group} (N: NormalSubgroup G) (H: Subgroup G)
-  : NormalSubgroup H := [subgrp N in H] <<| H.
+Program Definition NormalSubgroup_inSubgroup {G:Group} (N: NormalSubgroup G) (H: Subgroup G)
+  : NormalSubgroup H := < N inside H > <<| H.
 Next Obligation. split. intros g h. simpl. apply normal. Defined.
-Notation "[ 'nsgrp' N 'in' H ]" := (@nsg_in_sg _ N H).
+Notation "<|  N 'inside' H   |>" := (@NormalSubgroup_inSubgroup _ N H)
+  (at level 0, N, H at next level) : alg_scope.
 
 Program Definition HomImage `(f: Homomorph G H)
   : Map (Subgroup G) (Subgroup H)
-  := map A => grpable_as_sg ((Image f) (sg_as_grpable A)).
+  := map A => GroupableSubsetoid_toSubgroup ((Image f) (Subgroup_toGroupableSetoid A)).
 Next Obligation.
   split.
   - intros x y. simpl. intros [z1 [Az1 Heq1]] [z2 [Az2 Heq2]].
     exists (z1 * z2). split.
-    + apply (sg_ferm_op Az1 Az2).
+    + apply (ferm_op Az1 Az2).
     + now rewrite homomorph, Heq1, Heq2.
   - intros x [y [Ay Heq]].
-    exists !y. split.
-    + apply sg_ferm_inv, Ay.
+    exists (!y). split.
+    + apply ferm_inv, Ay.
     + now rewrite hom_inv, Heq.
   - exists 1. split.
-    + apply sg_ferm_id.
+    + apply ferm_id.
     + symmetry; apply hom_id.
 Defined.
 Next Obligation.
@@ -685,7 +707,7 @@ Next Obligation.
   - intros x y Heq1 Heq2.
     now rewrite homomorph, Heq1, Heq2, ridentical.
   - intros x Heq.
-    now rewrite hom_inv, Heq, grp_invid_id.
+    now rewrite hom_inv, Heq, invid.
   - apply hom_id.
 Defined.
 Next Obligation.
@@ -696,15 +718,15 @@ Defined.
 
 
 Program Definition Coset `(H: Subgroup G) :=
-  [setoid by fun x y => H (x * !y) on G].
+  std by fun x y => H (x * !y) on G.
 Next Obligation.
   split.
-  - intros x. rewrite rinvertible. apply sg_ferm_id.
-  - intros x y Heq. apply sg_ferm_inv in Heq.
-    now rewrite grp_opinv, grp_invinv in Heq.
+  - intros x. rewrite rinvertible. apply ferm_id.
+  - intros x y Heq. apply ferm_inv in Heq.
+    now rewrite opinv, invinv in Heq.
   - intros x y z Hxy Hyz.
-    pose (sg_ferm_op Hxy Hyz) as Hxz.
-    now rewrite associative, <-(associative x !y y), 
+    pose (ferm_op Hxy Hyz) as Hxz.
+    now rewrite associative, <-(associative x (!y) y), 
       linvertible, ridentical in Hxz.
 Defined.
 
@@ -716,73 +738,75 @@ Program Definition quotmap `{H: Subgroup G} : Map G (Coset H) :=
   map x => x.
 Next Obligation.
   split. intros x y Heq. simpl. rewrite Heq, rinvertible.
-  apply sg_ferm_id.
+  apply ferm_id.
 Defined.
 
 Lemma quotmap_surj `{H: Subgroup G} : Surjective (@quotmap G H).
 Proof.
   split. intros g. simpl. exists g. 
-  rewrite rinvertible. apply sg_ferm_id.
+  rewrite rinvertible. apply ferm_id.
 Defined.
 #[global]
 Existing Instance quotmap_surj.
 
 Program Definition CosetGroup `(H: NormalSubgroup G) :=
-  [group by (binop x, y => x * y), (map x => !x), 1 on Coset H].
+  grp by (binop x, y => x * y), (map x => !x), 1 on Coset H.
 Next Obligation.
   split. intros x0 y0. simpl. intros Heq0 x1 y1 Heq1.
   assert (H (x0 * x1 * !y1 * !x0)) as Heq2.
-  { rewrite <-(associative _ _ !y1). now apply normal. }
-  pose (sg_ferm_op Heq2 Heq0) as Heq3.
-  rewrite associative, <-(associative _ !x0 x0),
+  { rewrite <-(associative _ _ (!y1)). now apply normal. }
+  pose (ferm_op Heq2 Heq0) as Heq3.
+  rewrite associative, <-(associative _ (!x0) x0),
     linvertible, ridentical in Heq3.
-  now rewrite grp_opinv, associative.
+  now rewrite opinv, associative.
 Defined.
 Next Obligation.
-  split. intros x y. simpl. intros Heq. rewrite <-grp_opinv.
-  apply sg_ferm_inv. apply (normal(g := !y)) in Heq.
-  now rewrite grp_invinv, associative, <-(associative _ !y y),
+  split. intros x y. simpl. intros Heq. rewrite <-opinv.
+  apply ferm_inv. apply (normal(g := !y)) in Heq.
+  now rewrite invinv, associative, <-(associative _ (!y) y),
     linvertible, ridentical in Heq.
 Defined.
 Next Obligation.
   split; split.
   - intros x y z. simpl. rewrite associative, rinvertible.
-    apply sg_ferm_id.
-  - intros x. simpl. apply normal, sg_ferm_id.
-  - intros x. simpl. rewrite grp_invid_id, ridentical, rinvertible.
-    apply sg_ferm_id.
+    apply ferm_id.
+  - intros x. simpl. apply normal, ferm_id.
+  - intros x. simpl. rewrite invid, ridentical, rinvertible.
+    apply ferm_id.
 Defined.
-Notation "[ 'grp' G / N ]" := (@CosetGroup G N).
+Notation "<  G / N  >" := (@CosetGroup G N)
+  (at level 0, G, N at next level) : alg_scope.
 
 Program Definition quothom `{H: NormalSubgroup G}
-  : Homomorph G (CosetGroup H) := hom g => quotmap g.
+  : Homomorph G (CosetGroup H) := (hom g => (quotmap g)).
 Next Obligation. apply (map_prf _ _ quotmap). Defined.
 Next Obligation.
-  split. intros x y. simpl. rewrite rinvertible. apply sg_ferm_id.
+  split. intros x y. simpl. rewrite rinvertible. apply ferm_id.
 Defined.
+
 
 Section FundHom.
   Context {G H:Group} (f: Homomorph G H)
     (N := HomKernel f) (G_N := CosetGroup N).
 
   Program Definition Iso1_kernel {A: NormalSubgroup G} {B: Subgroup H}
-    (EAN: (A == N in Subgroup_setoid G))
-    (EBI: (B == HomImage f [subgrp {G}] in Subgroup_setoid H))
+    (EAN: (A == N in SubgroupSetoid G))
+    (EBI: (B == HomImage f <{ G }> in SubgroupSetoid H))
     : Isomorph (CosetGroup A) B :=
     iso x => f x.
   Next Obligation. apply H1. simpl. now exists x. Defined.
   Next Obligation.
     split. intros x y. simpl. intros Heq. apply i1 in Heq. simpl in Heq.
     rewrite homomorph, hom_inv in Heq.
-    apply grp_send_r in Heq.
-    now rewrite grp_invinv, lidentical in Heq.
+    apply send_r in Heq.
+    now rewrite invinv, lidentical in Heq.
   Defined.
   Next Obligation. split. intros x y. simpl. apply homomorph. Defined.
   Next Obligation.
     split; split; split.
     - intros x y. simpl. intros Heq. apply i2. simpl.
       rewrite homomorph, hom_inv.
-      symmetry; apply grp_send_r.
+      symmetry; apply send_r.
       now rewrite lidentical.
     - simpl. intros [y By]. simpl. destruct i as [i].
       simpl in i. destruct (i _ By) as [x [_ E]].
@@ -790,23 +814,23 @@ Section FundHom.
   Defined.
 
   Program Definition Iso1
-    : Isomorph G_N (HomImage f [subgrp {G}]) 
+    : Isomorph G_N (HomImage f <{ G }>) 
     := Iso1_kernel _ _.
   Next Obligation. split; split; intuition. Defined.
   Next Obligation. split; split; intuition. Defined.
 
   Lemma Iso1comp_proper :
-    f == inclusion \o Iso1 \o quotmap in (Map_setoid G H).
+    f == inclusion \o Iso1 \o quotmap in (MapSetoid G H).
   Proof. intros x y Heq. simpl. now rewrite Heq. Qed.
 
   Lemma Iso1_identical : forall (psi: Homomorph G_N H), 
-    f == psi \o quotmap in (Map_setoid G H) ->
-    psi == inclusion \o Iso1 in (Map_setoid G_N H).
+    f == psi \o quotmap in (MapSetoid G H) ->
+    psi == inclusion \o Iso1 in (MapSetoid G_N H).
   Proof.
     intros psi Hiso x y Heq. rewrite Heq.
     rewrite Iso1comp_proper in Hiso.
-    rewrite <-mapcomp_assoc in Hiso.
-    pose (mapcomp_reduc _ Hiso) as Heq2.
+    rewrite <-Map_assoc in Hiso.
+    pose (Map_reduc _ Hiso) as Heq2.
     symmetry. now apply Heq2.
   Qed.
 End FundHom.
@@ -815,8 +839,8 @@ Section CorrespSubgroup.
   Context {G:Group} {N: NormalSubgroup G} (G_N := CosetGroup N).
 
   Program Definition ExtendQuotGroups
-  : Map (Subgroup G_N) [substd of K in Subgroup G | N <= K]
-  := map H => grpable_as_sg (Preimage quotmap (sg_as_grpable H)).
+  : Map (Subgroup G_N) [ K in Subgroup G | N <= K ]
+  := map H => GroupableSubsetoid_toSubgroup (Preimage quotmap (Subgroup_toGroupableSetoid H)).
   Next Obligation.
     split. intros H1 H2. simpl. intros [H1H2 H2H1]. split; intros NH;
     now apply (transitivity NH).
@@ -824,16 +848,16 @@ Section CorrespSubgroup.
   Next Obligation.
     split.
     - intros g h. simpl. intros Hg Hh.
-      apply (sg_ferm_op(H := H) Hg Hh).
+      apply (ferm_op(H := H) Hg Hh).
     - intros g. simpl. intros Hg.
-      apply (sg_ferm_inv(H := H) Hg).
-    - apply (sg_ferm_id(H := H)).
+      apply (ferm_inv(H := H) Hg).
+    - apply (ferm_id(H := H)).
   Defined.
   Next Obligation.
     split. simpl. intros g Ng.
     assert (g == 1 in G_N) as Hid.
-    { simpl. now rewrite grp_invid_id, ridentical. }
-    rewrite Hid. apply (sg_ferm_id(H := H)).
+    { simpl. now rewrite invid, ridentical. }
+    rewrite Hid. apply (ferm_id(H := H)).
   Defined.
   Next Obligation.
     split. intros A B [AB BA]. split; split; intros x; simpl;
@@ -841,7 +865,7 @@ Section CorrespSubgroup.
   Defined.
 
   Program Definition FoldGroups
-    : Map [substd of K in Subgroup G | N <= K] (Subgroup G_N)
+    : Map [ K in Subgroup G | N <= K ] (Subgroup G_N)
     := map K => HomImage quothom K.
   Next Obligation.
     split. intros A B. simpl. intros [[AB] [BA]]. split; split;
@@ -862,11 +886,11 @@ Section CorrespSubgroup.
     intros [K1 N_K1] [K2 N_K2]. simpl. intros [[K12] [K21]]. split; split;
     intros g; simpl.
     - intros [h [K1h Eh]]. apply K12. apply N_K1 in Eh.
-      pose (sg_ferm_op Eh K1h) as K1g.
+      pose (ferm_op Eh K1h) as K1g.
       now rewrite <-associative, linvertible, ridentical in K1g.
     - intros K2g. exists g; split.
       + apply K21, K2g.
-      + rewrite rinvertible. apply sg_ferm_id.
+      + rewrite rinvertible. apply ferm_id.
   Defined.
 
   Lemma corresp_comp_id_qsg :
@@ -878,15 +902,15 @@ Section CorrespSubgroup.
       now rewrite (coset_eq Eh).
     - intros H2g. simpl. exists g. split.
       + now apply H21.
-      + rewrite rinvertible. apply sg_ferm_id.
+      + rewrite rinvertible. apply ferm_id.
   Defined.
 End CorrespSubgroup.
 
 
-Program Definition dprod_group (G H:Group):=
-  [group by binop g, h => (fst g * fst h, snd g * snd h),
+Program Definition DirectProductGroup (G H:Group):=
+  grp by binop g, h => (fst g * fst h, snd g * snd h),
             map g => (!(fst g), !(snd g)),
-            (1, 1) on [dprodstd G \* H]].
+            (1, 1) on [(G, H)].
 Next Obligation.
   split. intros g h [Heq0 Heq1] x y [Heq2 Heq3]. split; simpl.
   - now rewrite Heq0, Heq2.
@@ -905,41 +929,43 @@ Defined.
   (G, ) *)
 
 Program Definition sg_prod {G:Group} (H1 H2: Subgroup G) :=
-  [substd of g | exists h1 h2, H1 h1 /\ H2 h2 /\ g == h1 * h2].
+  [ g | exists h1 h2, H1 h1 /\ H2 h2 /\ g == h1 * h2 ].
 Next Obligation.
   split. intros x y Heq. split; 
   intros [h [n [Hh [Nn Heq1]]]]; exists h, n; split; 
   try split; try apply Hh; try apply Nn;
   now rewrite <-Heq1, Heq.
 Defined.
-Notation "[ 'substd' N \* H ]" := (@sg_prod _ N H).
+Notation "[  N * H  ]" := (@sg_prod _ N H)
+  (at level 0, N, H at next level, no associativity) : alg_scope.
 
 Program Definition sgnsg_prod `(H: Subgroup G) (N: NormalSubgroup G)
-  := [substd H \* N] <<- G.
+  := [ H * N ]  <<- G.
 Next Obligation.
   split; simpl.
   - intros x y [hx [nx [Hhx [Nnx Heqx]]]]
     [hy [ny [Hhy [Nny Heqy]]]]. 
     pose (normal(g := !hy) Nnx) as Heq0.
-    rewrite grp_invinv in Heq0. 
+    rewrite invinv in Heq0. 
     exists (hx * hy), (!hy * nx * hy * ny). split; try split.
-    + apply (sg_ferm_op Hhx Hhy).
-    + apply (sg_ferm_op Heq0 Nny).
+    + apply (ferm_op Hhx Hhy).
+    + apply (ferm_op Heq0 Nny).
     + now rewrite 3!associative, <-(associative hx),
         rinvertible, ridentical, Heqx, Heqy, associative.
   - intros x [h [n [Hh [Nn Heq]]]].
-    exists !h, (h * !n * !h). split; try split.
-    + apply sg_ferm_inv, Hh.
-    + apply normal, sg_ferm_inv, Nn.
+    exists (!h), (h * !n * !h). split; try split.
+    + apply ferm_inv, Hh.
+    + apply normal, ferm_inv, Nn.
     + now rewrite 2!associative, linvertible, lidentical, 
-        Heq, grp_opinv.
-  - exists 1, 1. split; try split; try apply sg_ferm_id.
+        Heq, opinv.
+  - exists 1, 1. split; try split; try apply ferm_id.
     now rewrite ridentical.
 Defined.
-Notation "[ 'subgrp' H *|> N ]" := (@sgnsg_prod _ H N).
+Notation "<  H *> N  >" := (@sgnsg_prod _ H N)
+  (at level 0, H, N at next level) : alg_scope.
 
 Lemma sg_prod_comm `{H: Subgroup G} {N: NormalSubgroup G} : 
-  [substd H \* N] == [substd N \* H] in Subsetoid_setoid G.
+  [ H * N ] == [ N * H ] in SubsetoidSetoid G.
 Proof.
   split; split; intros g [h1 [h2 [Hh1 [Hh2 Heq]]]]; simpl.
   - exists (h1 * h2 * !h1), h1; split; try split.
@@ -950,47 +976,48 @@ Proof.
     + trivial.
     + now apply normal.
     + now rewrite 2!associative, rinvertible, 
-        lidentical, grp_invinv.
+        lidentical, invinv.
 Qed.
 
 Lemma stdeq_grpable {G:Group} {A B: Subsetoid G}
   : A == B -> A <- G -> B <- G.
 Proof.
-  intros AB AG. assert ((Subgroupable_subsetoid G) A).
+  intros AB AG. assert ((GroupableSubsetoid G) A).
   { apply AG. } rewrite AB in H. apply H.
 Qed.
 
 Program Definition nsgsg_prod `(N: NormalSubgroup G) (H: Subgroup G)
-  := [substd N \* H] <<- G.
+  := [ N * H ] <<- G.
 Next Obligation.
   apply (stdeq_grpable sg_prod_comm), sgnsg_prod_obligation_1.
 Defined.
-Notation "[ 'subgrp' N <|* H ]" := (@nsgsg_prod _ N H).
+Notation "<  N <* H  >" := (@nsgsg_prod _ N H)
+  (at level 0, N, H at next level) : alg_scope.
 
 Program Definition Hom2 `{H: Subgroup G} {N: NormalSubgroup G}
-  : Homomorph H (CosetGroup [nsgrp N in [subgrp H *|> N]])
+  : Homomorph H (CosetGroup <| N inside < H *> N> |>)
   := hom g => g.
 Next Obligation.
   exists g, 1. split; try split.
   - apply H0.
-  - apply sg_ferm_id.
+  - apply ferm_id.
   - now rewrite ridentical.
 Defined.
 Next Obligation.
   split. intros g h. simpl. intros Heq. rewrite Heq, rinvertible.
-  apply sg_ferm_id.
+  apply ferm_id.
 Defined.
 Next Obligation.
-  split. intros g h. simpl. rewrite rinvertible. apply sg_ferm_id.
+  split. intros g h. simpl. rewrite rinvertible. apply ferm_id.
 Defined.
 
 Program Definition Iso2' `{H: Subgroup G} {N: NormalSubgroup G}
-  := (@Iso1_kernel _ _ Hom2 [nsgrp N in H]
-      [subgrp {CosetGroup [nsgrp N in [subgrp H *|> N]]}] _ _).
+  := (@Iso1_kernel _ _ Hom2 <| N inside H |>
+      <{ CosetGroup <| N inside <H *> N> |> }> _ _).
 Next Obligation.
   split; split; intros [h Hh]; simpl.
-  - intros Nh. now rewrite grp_invid_id, ridentical.
-  - intros E. now rewrite grp_invid_id, ridentical in E.
+  - intros Nh. now rewrite invid, ridentical.
+  - intros E. now rewrite invid, ridentical in E.
 Defined.
 Next Obligation.
   split; split; intros [g [h [n [Hh [Nn Eg]]]]]; simpl.
@@ -999,7 +1026,7 @@ Next Obligation.
   - split.
 Defined.
 
-Program Definition id_grpsg_iso {G:Group} : Isomorph G [subgrp {G}]
+Program Definition id_grpsg_iso {G:Group} : Isomorph G <{ G }>
   := iso g => g.
 Next Obligation. split. intros g h. simpl. intuition. Defined.
 Next Obligation. split. intros g h. simpl. reflexivity. Defined.
@@ -1007,8 +1034,8 @@ Next Obligation.
   split; split; split; simpl. intuition. intros [y Hy]. now exists y.
 Defined.
 
-Program Definition grpsg_id_iso {G:Group} : Isomorph [subgrp {G}] G
-  := iso g => g.
+Program Definition grpidNormalSubgroup_iso {G:Group}
+  : Isomorph <{ G }> G := iso g => g.
 Next Obligation. split. intros g h. simpl. intuition. Defined.
 Next Obligation. split. intros g h. simpl. reflexivity. Defined.
 Next Obligation. 
@@ -1016,9 +1043,9 @@ Next Obligation.
 Defined.
 
 Definition Iso2 `{H: Subgroup G} {N: NormalSubgroup G}
-  : Isomorph (CosetGroup [nsgrp N in H])
-    (CosetGroup [nsgrp N in [subgrp H *|> N]])
-  := grpsg_id_iso \o_i Iso2'.
+  : Isomorph (CosetGroup <| N inside H |>)
+    (CosetGroup <| N inside < H *> N > |>)
+  := grpidNormalSubgroup_iso iso\o Iso2'.
 
 
 Program Definition Hom3 {G:Group} {N1 N2: NormalSubgroup G} (Hle: N1 <= N2)
@@ -1026,45 +1053,45 @@ Program Definition Hom3 {G:Group} {N1 N2: NormalSubgroup G} (Hle: N1 <= N2)
   :=  hom g in CosetGroup N1 => g.
 Next Obligation. split. intros g h. simpl. apply Hle. Defined.
 Next Obligation.
-  split. intros g h. simpl. rewrite rinvertible. apply sg_ferm_id.
+  split. intros g h. simpl. rewrite rinvertible. apply ferm_id.
 Defined.
 
 Program Definition coset_nsg {G} {N1 N2: NormalSubgroup G} (Hle: N1 <= N2)
-  := [substd by N2 on CosetGroup N1] <<-| (CosetGroup N1).
+  := (sstd by N2 on CosetGroup N1) <<-| (CosetGroup N1).
 Next Obligation.
-split. intros g h. simpl. intros Egh. split; intros Ng.
-- apply Hle in Egh. apply sg_ferm_inv in Egh.
-  rewrite grp_opinv, grp_invinv in Egh.
-  pose (sg_ferm_op Egh Ng) as N2h.
-  now rewrite <-associative, linvertible, ridentical in N2h.
-- apply Hle in Egh. pose (sg_ferm_op Egh Ng) as N2g.
-  now rewrite <-associative, linvertible, ridentical in N2g.
+  split. intros g h. simpl. intros Egh. split; intros Ng.
+  - apply Hle in Egh. apply ferm_inv in Egh.
+    rewrite opinv, invinv in Egh.
+    pose (ferm_op Egh Ng) as N2h.
+    now rewrite <-associative, linvertible, ridentical in N2h.
+  - apply Hle in Egh. pose (ferm_op Egh Ng) as N2g.
+    now rewrite <-associative, linvertible, ridentical in N2g.
 Defined.
 Next Obligation.
-split.
-- intros g h. simpl. apply sg_ferm_op.
-- intros g. simpl. apply sg_ferm_inv.
-- simpl. apply sg_ferm_id.
+  split.
+  - intros g h. simpl. apply ferm_op.
+  - intros g. simpl. apply ferm_inv.
+  - simpl. apply ferm_id.
 Defined.
 Next Obligation. split. intros g h. simpl. apply normal. Defined.
-Notation "[ 'subgrp' H / N ]" := (@coset_nsg _ N H _).
+Notation "<| H /> N |>" := (@coset_nsg _ N H _)
+  (at level 0, H, N at next level) : alg_scope.
 
 Program Definition Iso3' {G:Group} {N1 N2: NormalSubgroup G} (Hle: N1 <= N2)
-  := (@Iso1_kernel _ _ (Hom3 Hle) (coset_nsg Hle) [subgrp {CosetGroup N2}] _ _).
+  := (@Iso1_kernel _ _ (Hom3 Hle) (coset_nsg Hle) <{ CosetGroup N2 }> _ _).
 Next Obligation.
   split; split; intros g; simpl; intros N2g.
-  - now rewrite grp_invid_id, ridentical.
-  - now rewrite grp_invid_id, ridentical in N2g.
+  - now rewrite invid, ridentical.
+  - now rewrite invid, ridentical in N2g.
 Defined.
 Next Obligation.
   split; split; intros g; simpl; intuition. exists g.
-  split; trivial. rewrite rinvertible. apply sg_ferm_id.
+  split; trivial. rewrite rinvertible. apply ferm_id.
 Defined.
 
 Definition Iso3 {G:Group} {N1 N2: NormalSubgroup G} (Hle: N1 <= N2)
-  : Isomorph (CosetGroup (coset_nsg _)) (CosetGroup N2)
-  := grpsg_id_iso \o_i (Iso3' Hle).
+  : Isomorph (CosetGroup <| N2 /> N1 |>) (CosetGroup N2)
+  := grpidNormalSubgroup_iso iso\o (Iso3' Hle).
 
 Close Scope alg_scope.
 Close Scope setoid_scope.
-
